14MachineCode/Disassemble.thy
@@ -7,21 +7,18 @@ primrec register_map :: "register \<Rightarrow> reg" where
 | "register_map Env = R2"
 | "register_map Vals = R3"
 | "register_map Stk = R4"
-| "register_map Acc = R5"
 
 primrec register_offset :: "register \<Rightarrow> nat" where
   "register_offset Hp = 0"
 | "register_offset Env = 1"
 | "register_offset Vals = 2"
 | "register_offset Stk = 3"
-| "register_offset Acc = 0"
 
 primrec register_size :: "register \<Rightarrow> nat" where
   "register_size Hp = 4"
 | "register_size Env = 4"
 | "register_size Vals = 4"
 | "register_size Stk = 4"
-| "register_size Acc = 1"
 
 primrec pseudoreg_size :: "pseudoreg \<Rightarrow> nat" where
   "pseudoreg_size (Reg r) = register_size r"
@@ -32,14 +29,16 @@ fun disassemble' :: "assm \<Rightarrow> mach" where
   "disassemble' (AMov (Reg r)) = MOV R5 (register_map r)"
 | "disassemble' (AMov PC) = MVP R5"
 | "disassemble' (AMov (Con k)) = LDI R5 k"
-| "disassemble' (AGet r1 r2 t) = LOD R5 (register_map r2)"
-| "disassemble' (APut r1 r2 (Reg r3)) = STO (register_map r1) (register_map r3)"
-| "disassemble' (APut r1 r2 PC) = undefined"
-| "disassemble' (APut r1 r2 (Con k)) = STI (register_map r1) k"
-| "disassemble' (ASub Acc k t) = SUB R5 (pseudoreg_size t * k)"
-| "disassemble' (ASub r k t) = SUB (register_map r) (4 * k)"
-| "disassemble' (AAdd Acc k t) = ADD R5 (pseudoreg_size t * k)"
-| "disassemble' (AAdd r k t) = ADD (register_map r) (4 * k)"
+| "disassemble' (AGetA r t) = LOD R5 (register_map r)"
+| "disassemble' (AGet r t) = LOD R5 (register_map r)"
+| "disassemble' (APutA r) = STO (register_map r) R5"
+| "disassemble' (APut r (Reg r')) = STO (register_map r) (register_map r')"
+| "disassemble' (APut r PC) = undefined"
+| "disassemble' (APut r (Con k)) = STI (register_map r) k"
+| "disassemble' (ASubA k t) = SUB R5 (pseudoreg_size t * k)"
+| "disassemble' (ASub r k) = SUB (register_map r) (4 * k)"
+| "disassemble' (AAddA k t) = ADD R5 (pseudoreg_size t * k)"
+| "disassemble' (AAdd r k) = ADD (register_map r) (4 * k)"
 | "disassemble' AJmp = JMP R5"
 
 definition disassemble :: "assm list \<Rightarrow> mach list" where
@@ -55,20 +54,35 @@ fun unmap_mem' :: "nat \<Rightarrow> register \<times> nat" where
 definition unmap_mem :: "(register \<Rightarrow> nat \<Rightarrow> nat) \<Rightarrow> nat \<Rightarrow> nat" where
   "unmap_mem m x = (case unmap_mem' x of (r, p) \<Rightarrow> m r p)"
 
-fun inv_register_map :: "(register \<Rightarrow> nat) \<Rightarrow> pseudoreg \<Rightarrow> reg \<Rightarrow> nat" where
-  "inv_register_map rs t R1 = rs Hp * 4"
-| "inv_register_map rs t R2 = rs Env * 4 + 1"
-| "inv_register_map rs t R3 = rs Vals * 4 + 2"
-| "inv_register_map rs t R4 = rs Stk * 4 + 3"
-| "inv_register_map rs (Reg r) R5 = rs Acc * 4 + register_offset r"
-| "inv_register_map rs PC R5 = rs Acc"
-| "inv_register_map rs (Con k) R5 = rs Acc"
+fun inv_register_map :: "(register \<Rightarrow> nat) \<Rightarrow> nat \<Rightarrow> pseudoreg \<Rightarrow> reg \<Rightarrow> nat" where
+  "inv_register_map rs a t R1 = rs Hp * 4"
+| "inv_register_map rs a t R2 = rs Env * 4 + 1"
+| "inv_register_map rs a t R3 = rs Vals * 4 + 2"
+| "inv_register_map rs a t R4 = rs Stk * 4 + 3"
+| "inv_register_map rs a (Reg r) R5 = a * 4 + register_offset r"
+| "inv_register_map rs a PC R5 = a"
+| "inv_register_map rs a (Con k) R5 = a"
 
 primrec disassemble_state :: "assm_state \<Rightarrow> mach_state" where
-  "disassemble_state (AS mem rs t pc) = MS (inv_register_map rs t) (unmap_mem mem) pc"
+  "disassemble_state (AS mem rs a t pc) = MS (inv_register_map rs a t) (unmap_mem mem) pc"
 
 primrec dissassembleable :: "assm_state \<Rightarrow> nat \<Rightarrow> bool" where
-  "dissassembleable (AS mem rs t pc) lcd = (pc < lcd)"
+  "dissassembleable (AS mem rs a t pc) lcd = (pc < lcd)"
+
+lemma [dest]: "R1 = register_map r \<Longrightarrow> r = Hp"
+  by (induction r) simp_all
+
+lemma [dest]: "R2 = register_map r \<Longrightarrow> r = Env"
+  by (induction r) simp_all
+
+lemma [dest]: "R3 = register_map r \<Longrightarrow> r = Vals"
+  by (induction r) simp_all
+
+lemma [dest]: "R4 = register_map r \<Longrightarrow> r = Stk"
+  by (induction r) simp_all
+
+lemma [dest]: "R5 = register_map r \<Longrightarrow> False"
+  by (induction r) simp_all
 
 lemma [simp]: "unmap_mem' (4 * k) = (Hp, k)"
   by (induction k) (simp_all add: numeral_def)
@@ -111,32 +125,29 @@ next
   thus ?case by simp
 qed
 
-lemma inv_reg_map_reg: "r \<noteq> Acc \<Longrightarrow> 
-  (inv_register_map ps act)(R5 := inv_register_map ps act (register_map r)) = 
-    inv_register_map (ps(Acc := ps r)) (Reg r)"
+lemma inv_reg_map_reg: "(inv_register_map ps a act)(R5 := inv_register_map ps a act (register_map r)) = 
+  inv_register_map ps (ps r) (Reg r)"
 proof
   fix x
-  show "r \<noteq> Acc \<Longrightarrow> 
-    ((inv_register_map ps act)(R5 := inv_register_map ps act (register_map r))) x = 
-      inv_register_map (ps(Acc := ps r)) (Reg r) x"
+  show "((inv_register_map ps a act)(R5 := inv_register_map ps a act (register_map r))) x = 
+      inv_register_map ps (ps r) (Reg r) x"
   proof (induction x)
     case R5
     thus ?case by (induction r) simp_all
   qed simp_all
 qed
 
-lemma inv_reg_map_pc: "(inv_register_map ps act)(R5 := pc) = inv_register_map (ps(Acc := pc)) PC"
+lemma inv_reg_map_pc: "(inv_register_map ps a act)(R5 := pc) = inv_register_map ps pc PC"
 proof
   fix x
-  show "((inv_register_map ps act)(R5 := pc)) x = inv_register_map (ps(Acc := pc)) PC x"
+  show "((inv_register_map ps a act)(R5 := pc)) x = inv_register_map ps pc PC x"
     by (induction x) simp_all
 qed
 
-lemma inv_reg_map_con: "(inv_register_map ps act)(R5 := k) = 
-  inv_register_map (ps(Acc := k)) (Con 0)"
+lemma inv_reg_map_con: "(inv_register_map ps a act)(R5 := k) = inv_register_map ps k (Con 0)"
 proof
   fix x
-  show "((inv_register_map ps act)(R5 := k)) x = inv_register_map (ps(Acc := k)) (Con 0) x"
+  show "((inv_register_map ps a act)(R5 := k)) x = inv_register_map ps k (Con 0) x"
     by (induction x) simp_all
 qed
 
@@ -152,153 +163,97 @@ lemma [simp]: "unmap_mem' (Suc (Suc (k * 4))) = (Vals, k)"
 lemma [simp]: "unmap_mem' (k * 4 + 3) = (Stk, k)"
   by (induction k) (simp_all add: numeral_def)
 
-lemma [simp]: "m \<noteq> Acc \<Longrightarrow> unmap_mem' (k * 4 + register_offset m) = (m, k)"
+lemma [simp]: "unmap_mem' (k * 4 + register_offset m) = (m, k)"
 proof (induction k)
   case 0
   thus ?case by (induction m) (simp_all add: numeral_def)
 qed (simp_all add: numeral_def)
 
-lemma [simp]: "r \<noteq> Acc \<Longrightarrow> inv_register_map (ps(r := k)) act R5 = inv_register_map ps act R5"
+lemma [simp]: "inv_register_map (ps(r := k)) a act R5 = inv_register_map ps a act R5"
   by (induction act) simp_all
 
-lemma [simp]: "r \<noteq> Acc \<Longrightarrow> inv_register_map (ps(r := ps r + k)) act = 
-    ((inv_register_map ps act)(register_map r := inv_register_map ps act (register_map r) + 4 * k))"
+lemma [simp]: "inv_register_map (ps(r := ps r + k)) a act = 
+  ((inv_register_map ps a act)
+    (register_map r := inv_register_map ps a act (register_map r) + 4 * k))"
 proof
   fix x
-  show "r \<noteq> Acc \<Longrightarrow> inv_register_map (ps(r := ps r + k)) act x =
-    ((inv_register_map ps act)(register_map r := inv_register_map ps act (register_map r) + 4 * k)) 
-      x" 
-  proof (induction r)
-    case Hp
-    thus ?case by (induction x) simp_all
-  next
-    case Env
-    thus ?case by (induction x) simp_all
-  next
-    case Vals
-    thus ?case by (induction x) simp_all
-  next
-    case Stk
-    thus ?case by (induction x) simp_all
-  next
-    case Acc
-    thus ?case by (induction x) simp_all
-  qed
+  show "inv_register_map (ps(r := ps r + k)) a act x =
+    ((inv_register_map ps a act)
+      (register_map r := inv_register_map ps a act (register_map r) + 4 * k)) x" 
+    by (induction ps a act x rule: inv_register_map.induct) auto
 qed
 
-lemma [simp]: "r \<noteq> Acc \<Longrightarrow> inv_register_map (ps(r := ps r - k)) act = 
-    ((inv_register_map ps act)(register_map r := inv_register_map ps act (register_map r) - 4 * k))"
+lemma [simp]: "inv_register_map (ps(r := ps r - k)) a act = 
+  ((inv_register_map ps a act)
+    (register_map r := inv_register_map ps a act (register_map r) - 4 * k))"
 proof
   fix x
-  show "r \<noteq> Acc \<Longrightarrow> inv_register_map (ps(r := ps r - k)) act x =
-    ((inv_register_map ps act)(register_map r := inv_register_map ps act (register_map r) - 4 * k)) 
-      x" 
-  proof (induction r)
-    case Hp
-    thus ?case by (induction x) simp_all
-  next
-    case Env
-    thus ?case by (induction x) simp_all
-  next
-    case Vals
-    thus ?case by (induction x) simp_all
-  next
-    case Stk
-    thus ?case by (induction x) simp_all
-  next
-    case Acc
-    thus ?case by (induction x) simp_all
-  qed
+  show "inv_register_map (ps(r := ps r - k)) a act x =
+    ((inv_register_map ps a act)
+      (register_map r := inv_register_map ps a act (register_map r) - 4 * k)) x" 
+    by (induction ps a act x rule: inv_register_map.induct) auto
 qed
 
-lemma [simp]: "m \<noteq> Acc \<Longrightarrow> (r \<noteq> Acc \<Longrightarrow> m = r) \<Longrightarrow>
-    unmap_mem mem (inv_register_map ps (Reg m) (register_map r)) = mem m (ps r)"
+lemma [simp]: "unmap_mem mem (inv_register_map ps a (Reg r) (register_map r)) = mem r (ps r)"
   by (induction r) (simp_all add: unmap_mem_def split: prod.splits)
 
-lemma [simp]: "m \<noteq> Acc \<Longrightarrow> unmap_mem mem (ps Acc * 4 + register_offset m) = mem m (ps Acc)"
+lemma [simp]: "unmap_mem mem (a * 4 + register_offset m) = mem m a"
   by (simp add: unmap_mem_def)
 
-lemma [simp]: "Suc pc < length cd \<Longrightarrow> disassemble cd ! pc = disassemble' (cd ! pc)"
+lemma [simp]: "lookup cd pc = Some op \<Longrightarrow> disassemble cd ! pc = disassemble' op"
 proof (induction cd)
   case (Cons op cd)
   thus ?case by (induction pc) (simp_all add: disassemble_def)
 qed simp_all
 
-theorem correctm [simp]: "cd\<^sub>a \<tturnstile> \<Sigma>\<^sub>a \<leadsto>\<^sub>a \<Sigma>\<^sub>a' \<Longrightarrow> dissassembleable \<Sigma>\<^sub>a (length cd\<^sub>a) \<Longrightarrow>
+theorem correctm [simp]: "cd\<^sub>a \<tturnstile> \<Sigma>\<^sub>a \<leadsto>\<^sub>a \<Sigma>\<^sub>a' \<Longrightarrow> 
   disassemble cd\<^sub>a \<tturnstile> disassemble_state \<Sigma>\<^sub>a \<leadsto>\<^sub>m disassemble_state \<Sigma>\<^sub>a'"
 proof (induction cd\<^sub>a \<Sigma>\<^sub>a \<Sigma>\<^sub>a' rule: evala.induct)
-  case (eva_movr cd pc r mem ps act)
-  hence "disassemble cd \<tturnstile> MS (inv_register_map ps act) (unmap_mem mem) (Suc pc) \<leadsto>\<^sub>m
-    MS ((inv_register_map ps act)(R5 := inv_register_map ps act (register_map r))) 
-      (unmap_mem mem) pc" by simp
-  with eva_movr show ?case by (simp add: inv_reg_map_reg)
-next
-  case (eva_movp cd pc mem ps act)
-  hence "disassemble cd \<tturnstile> MS (inv_register_map ps act) (unmap_mem mem) (Suc pc) \<leadsto>\<^sub>m
-    MS ((inv_register_map ps act)(R5 := pc)) (unmap_mem mem) pc" by simp
-  thus ?case by (simp add: inv_reg_map_pc)
-next
-  case (eva_movk cd pc k mem ps act)
-  hence "disassemble cd \<tturnstile> MS (inv_register_map ps act) (unmap_mem mem) (Suc pc) \<leadsto>\<^sub>m
-    MS ((inv_register_map ps act)(R5 := k)) (unmap_mem mem) pc" by simp
-  thus ?case by (simp add: inv_reg_map_con)
-next
-  case (eva_geta cd pc m t mem ps)
-  hence "disassemble cd ! pc = LOD R5 R5" by simp
-  hence "disassemble cd \<tturnstile> MS (inv_register_map ps (Reg m)) (unmap_mem mem) (Suc pc) \<leadsto>\<^sub>m 
-    MS ((inv_register_map ps (Reg m))(R5 := unmap_mem mem (inv_register_map ps (Reg m) R5))) 
-      (unmap_mem mem) pc" by (metis evm_lod)
-
-  with eva_geta have  "disassemble cd \<tturnstile> 
-    MS (inv_register_map ps (Reg m)) (unmap_mem mem) (Suc pc) \<leadsto>\<^sub>m
-      MS (inv_register_map (ps(Acc := mem m (ps Acc))) t) (unmap_mem mem) pc" by simp
-  thus ?case by simp
-next
-  case (eva_get cd pc r t mem ps act)
+  case (eva_movr cd pc r mem ps a act)
   then show ?case try0 by simp
 next
-  case (eva_putr cd pc m r' r mem ps act)
+  case (eva_movp cd pc mem ps a act)
   then show ?case try0 by simp
 next
-  case (eva_putp cd pc m r' mem ps act)
+  case (eva_movk cd pc k mem ps a act)
   then show ?case try0 by simp
 next
-  case (eva_putk cd pc m r' k mem ps act)
+  case (eva_geta cd pc m t mem ps a)
   then show ?case try0 by simp
 next
-  case (eva_suba cd pc k mem ps act)
+  case (eva_get cd pc r t mem ps a act)
   then show ?case try0 by simp
 next
-  case (eva_sub cd pc r k mem ps act)
-  hence "disassemble cd ! pc = SUB (register_map r) (4 * k)" by (cases r) simp_all
-  with eva_sub show ?case by simp
+  case (eva_puta cd pc r mem ps a act)
+  then show ?case try0 by simp
 next
-  case (eva_adda cd pc k act mem ps)
-  hence "disassemble cd \<tturnstile> MS (inv_register_map ps act) (unmap_mem mem) (Suc pc) \<leadsto>\<^sub>m
-    MS ((inv_register_map ps act)(R5 := inv_register_map ps act R5 + pseudoreg_size act * k)) 
-      (unmap_mem mem) pc" by simp
-  thus ?case by simp
+  case (eva_putr cd pc r r' mem ps a act)
+  then show ?case try0 by simp
 next
-  case (eva_add cd pc r k mem ps act)
-  hence "disassemble cd ! pc = ADD (register_map r) (4 * k)" by (cases r) simp_all
-  with eva_add show ?case by simp
+  case (eva_putp cd pc r mem ps a act)
+  then show ?case try0 by simp
 next
-  case (eva_jmp cd pc mem ps)
-  hence "disassemble cd ! pc = JMP R5" by simp
-  hence "disassemble cd \<tturnstile> MS (inv_register_map ps PC) (unmap_mem mem) (Suc pc) \<leadsto>\<^sub>m
-    MS ((inv_register_map ps PC)(R5 := 0)) (unmap_mem mem) (inv_register_map ps PC R5)" 
-      by (metis evm_jmp)
-  thus ?case by (simp add: inv_reg_map_con)
-qed
+  case (eva_putk cd pc r k mem ps a act)
+  then show ?case try0 by simp
+next
+  case (eva_suba cd pc k act mem ps a)
+  then show ?case try0 by simp
+next
+  case (eva_adda cd pc k act mem ps a)
+  then show ?case try0 by simp
+next
+  case (eva_jmp cd pc mem ps a)
+  then show ?case try0 by simp
+qed simp_all
 
 theorem correctm_iter [simp]: "iter (\<tturnstile> cd\<^sub>a \<leadsto>\<^sub>a) \<Sigma>\<^sub>a \<Sigma>\<^sub>a' \<Longrightarrow> 
     iter (\<tturnstile> disassemble cd\<^sub>a \<leadsto>\<^sub>m) (disassemble_state \<Sigma>\<^sub>a) (disassemble_state \<Sigma>\<^sub>a')"
-  by (induction \<Sigma>\<^sub>a \<Sigma>\<^sub>a' rule: iter.induct) (simp, metisx correctm iter_append iter_one)
+  by (induction \<Sigma>\<^sub>a \<Sigma>\<^sub>a' rule: iter.induct) (simp, metis correctm iter_append iter_one)
  
-lemma [simp]: "inv_register_map (case_register 0 0 0 2 0) (Con 0) = case_reg 0 1 2 11 0" 
+lemma [simp]: "inv_register_map (case_register 0 0 0 2) 0 (Con 0) = case_reg 0 1 2 11 0" 
   by (auto split: reg.splits)
 
-lemma [simp]: "inv_register_map (case_register hp ep (Suc 0) 0 0) (Con 0) = 
+lemma [simp]: "inv_register_map (case_register hp ep (Suc 0) 0) 0 (Con 0) = 
     case_reg (4 * hp) (Suc (4 * ep)) 6 3 0"
   by (auto split: reg.splits)
 
@@ -314,11 +269,11 @@ lemma [simp]: "unmap_mem' 7 = (Stk, 1)"
 lemma [dest]: "unmap_mem' x = (Stk, Suc 0) \<Longrightarrow> x = 7"
   by (induction x rule: unmap_mem'.induct) (auto split: prod.splits)
 
-lemma [simp]: "unmap_mem (case_register nmem nmem nmem (nmem(0 := 0, Suc 0 := 0)) nmem) = 
+lemma [simp]: "unmap_mem (case_register nmem nmem nmem (nmem(0 := 0, Suc 0 := 0))) = 
     (nmem(3 := 0, 7 := 0))"
   by rule (auto simp add: unmap_mem_def split: prod.splits register.splits)
 
-lemma [simp]: "unmap_mem (case_register h e v s nmem) 2 = v 0"
+lemma [simp]: "unmap_mem (case_register h e v s) 2 = v 0"
   by (simp add: unmap_mem_def numeral_def)
 
 end
