Correctness.thy
@@ -86,21 +86,21 @@ proof -
     (US h\<^sub>u hp\<^sub>u e\<^sub>u ep\<^sub>u vs\<^sub>u 1 sh\<^sub>u 0 0)" by simp
   let ?cd' = "assemble_code ?cd"
   let ?mp = "assembly_map ?cd"
-  let ?mem = "case_register (assm_hp hp\<^sub>u ?cd h\<^sub>u) e\<^sub>u vs\<^sub>u sh\<^sub>u nmem"
-  let ?rs = "case_register hp\<^sub>u ep\<^sub>u (Suc 0) 0 0"
+  let ?mem = "case_register (assm_hp hp\<^sub>u ?cd h\<^sub>u) e\<^sub>u vs\<^sub>u sh\<^sub>u"
+  let ?rs = "case_register hp\<^sub>u ep\<^sub>u (Suc 0) 0"
   from R EU have "iter (\<tturnstile> ?cd' \<leadsto>\<^sub>a) 
     (assemble_state ?mp (US nmem 0 nmem 0 nmem 0 (nmem(0 := 0, 1 := 0)) 2 (length ?cd))) 
       (assemble_state ?mp (US h\<^sub>u hp\<^sub>u e\<^sub>u ep\<^sub>u vs\<^sub>u 1 sh\<^sub>u 0 0))" by (metis correcta_iter)
   hence "iter (\<tturnstile> ?cd' \<leadsto>\<^sub>a) (AS (case_register (assm_hp 0 ?cd nmem) nmem nmem 
-    (nmem(0 := 0, 1 := 0)) nmem) (case_register 0 0 0 2 0) (Con 0) (length ?cd')) 
-      (AS ?mem ?rs (Con 0) 0)" by simp 
+    (nmem(0 := 0, 1 := 0))) (case_register 0 0 0 2) 0 (Con 0) (length ?cd')) 
+      (AS ?mem ?rs 0 (Con 0) 0)" by simp 
   hence "iter (\<tturnstile> disassemble ?cd' \<leadsto>\<^sub>m) 
     (disassemble_state (AS (case_register (assm_hp 0 ?cd nmem) nmem nmem 
-      (nmem(0 := 0, 1 := 0)) nmem) (case_register 0 0 0 2 0) (Con 0) (length ?cd')))
-        (disassemble_state (AS ?mem ?rs (Con 0) 0))" by (metis correctm_iter)
+      (nmem(0 := 0, 1 := 0))) (case_register 0 0 0 2) 0 (Con 0) (length ?cd')))
+        (disassemble_state (AS ?mem ?rs 0 (Con 0) 0))" by (metis correctm_iter)
   hence "iter (\<tturnstile> disassemble ?cd' \<leadsto>\<^sub>m) (MS (case_reg 0 1 2 11 0)
-    (unmap_mem (case_register (assm_hp 0 ?cd nmem) nmem nmem (nmem(0 := 0, Suc 0 := 0)) 
-      nmem)) (list_sum (map assemble_op_len ?cd)))
+    (unmap_mem (case_register (assm_hp 0 ?cd nmem) nmem nmem (nmem(0 := 0, Suc 0 := 0)))) 
+      (list_sum (map assemble_op_len ?cd)))
         (MS (case_reg (4 * hp\<^sub>u) (Suc (4 * ep\<^sub>u)) 6 3 0) (unmap_mem ?mem) 0)" 
     by simp
   with C T have EM: "iter (\<tturnstile> cd \<leadsto>\<^sub>m) (MS (case_reg 0 1 2 11 0) (nmem(3 := 0, 7 := 0)) (length cd)) 
